A draft design of an inclusive MSI protocol

src/Ex/Msi.v
@@ -1,9 +1,13 @@
-Require Import Bool Vector List String Peano_dec.
+Require Import Bool Vector List String Peano_dec Lia.
 Require Import Common FMap HVector ListSupport.
 
 Require Import Ex.Spec.
 
 Set Implicit Arguments.
+
+Local Open Scope list.
+Local Open Scope hvec.
+Local Open Scope fmap.
 
 (** Message Ids *)
 
@@ -23,6 +27,10 @@ Definition msiInvRq: IdxT := 2~>4.
 Definition msiInvWRq: IdxT := 2~>5.
 Definition msiInvRs: IdxT := 2~>6.
 
+(* Only used in inclusive cache-coherence protocols *)
+Definition msiBInvRq: IdxT := 3~>0.
+Definition msiBInvRs: IdxT := 3~>1.
+
 (** Cache Status *)
 
 Notation MSI := nat (only parsing).
@@ -31,3 +39,253 @@ Definition msiS: MSI := 2.
 Definition msiI: MSI := 1.
 Definition msiNP: MSI := 0. (* Not Present *)
 
+Section Invalidate.
+  Definition invalidate (st: MSI) :=
+    if eq_nat_dec st msiNP then msiNP else msiI.
+
+  Lemma invalidate_sound:
+    forall st, invalidate st <= msiI.
+  Proof. unfold invalidate; cbv; intros; find_if_inside; lia. Qed.
+
+  Lemma invalidate_I:
+    forall st, msiI <= st -> invalidate st = msiI.
+  Proof. unfold invalidate; cbv; intros; find_if_inside; lia. Qed.
+
+  Lemma invalidate_NP:
+    forall st, st = msiNP -> invalidate st = msiNP.
+  Proof. unfold invalidate; cbv; intros; find_if_inside; lia. Qed.
+End Invalidate.
+
+Hint Resolve invalidate_sound.
+
+Ltac solve_msi :=
+  unfold msiM, msiS, msiI, msiNP in *; solve [auto|lia].
+
+Definition val: Fin.t 4 := F1.
+Definition owned: Fin.t 4 := F2.
+Definition status: Fin.t 4 := F3.
+Definition dir: Fin.t 4 := F4.
+
+Section Directory.
+
+  Record DirT: Set :=
+    { dir_st: MSI; (* the summary status of children *)
+      dir_excl: IdxT;
+      dir_sharers: list IdxT
+    }.
+
+  Definition dirInit: DirT :=
+    {| dir_st := msiI;
+       dir_excl := ii;
+       dir_sharers := nil |}.
+
+  Import CaseNotations.
+  Definition getDir (oidx: IdxT) (dir: DirT): MSI :=
+    match case dir.(dir_st) on eq_nat_dec default msiI with
+    | msiM: if idx_dec oidx dir.(dir_excl) then msiM else msiI
+    | msiS: if in_dec idx_dec oidx dir.(dir_sharers)
+            then msiS else msiI
+    end.
+
+  Definition setDirM (oidx: IdxT) :=
+    {| dir_st := msiM;
+       dir_excl := oidx;
+       dir_sharers := nil |}.
+
+  Definition setDirS (oinds: list IdxT) :=
+    {| dir_st := msiS;
+       dir_excl := 0;
+       dir_sharers := oinds |}.
+
+  Definition setDirI :=
+    {| dir_st := msiI;
+       dir_excl := 0;
+       dir_sharers := nil |}.
+
+  Definition addSharer (oidx: IdxT) (dir: DirT): DirT :=
+    {| dir_st := msiS;
+       dir_excl := dir.(dir_excl);
+       dir_sharers :=
+         if eq_nat_dec dir.(dir_st) msiS
+         then oidx :: dir.(dir_sharers) else [oidx] |}.
+
+  Definition removeSharer (oidx: IdxT) (dir: DirT): DirT :=
+    {| dir_st := msiS;
+       dir_excl := dir.(dir_excl);
+       dir_sharers := removeOnce idx_dec oidx dir.(dir_sharers) |}.
+
+  Definition LastSharer (dir: DirT) (cidx: IdxT) :=
+    dir.(dir_sharers) = [cidx].
+
+  Definition NotLastSharer (dir: DirT) :=
+    2 <= List.length dir.(dir_sharers).
+
+  Definition OtherSharerExists (dir: DirT) (cidx: IdxT) :=
+    remove idx_dec cidx dir.(dir_sharers) <> nil.
+
+  Section Facts.
+
+    Ltac dir_crush :=
+      cbv [getDir addSharer removeSharer
+                  setDirI setDirS setDirM];
+      simpl; intros;
+      repeat find_if_inside;
+      repeat
+        (try match goal with
+             | [H: ~ In ?oidx (?oidx :: _) |- _] => elim H; left; reflexivity
+             | [Ht: In ?oidx ?l, Hn: ~ In ?oidx (_ :: ?l) |- _] => elim Hn; right; assumption
+             | [H: In _ (_ :: _) |- _] => inv H
+             | [H: _ |- _] => exfalso; auto; fail
+             end; try subst; try reflexivity; try assumption; try solve_msi).
+
+    Lemma getDir_M_imp:
+      forall oidx dir,
+        getDir oidx dir = msiM ->
+        dir.(dir_st) = msiM /\ dir.(dir_excl) = oidx.
+    Proof.
+      unfold getDir, caseDec; intros.
+      find_if_inside; [find_if_inside; [auto|discriminate]|].
+      repeat (find_if_inside; [find_if_inside; discriminate|]).
+      discriminate.
+    Qed.
+
+    Lemma getDir_S_imp:
+      forall oidx dir,
+        getDir oidx dir = msiS ->
+        dir.(dir_st) = msiS /\ In oidx dir.(dir_sharers).
+    Proof.
+      unfold getDir, caseDec; intros.
+      repeat (find_if_inside; [find_if_inside; discriminate|]).
+      find_if_inside; [find_if_inside; [auto|discriminate]|].
+      discriminate.
+    Qed.
+
+    Lemma getDir_addSharer_spec:
+      forall dir,
+        dir.(dir_st) <= msiS ->
+        forall oidx sidx,
+          getDir oidx (addSharer sidx dir) =
+          if idx_dec sidx oidx
+          then msiS else getDir oidx dir.
+    Proof. dir_crush. Qed.
+
+    Lemma getDir_removeSharer_sound:
+      forall oidx sidx dir,
+        getDir oidx (removeSharer sidx dir) <= msiS.
+    Proof. dir_crush. Qed.
+
+    Lemma getDir_removeSharer_neq:
+      forall oidx sidx dir,
+        getDir sidx dir = msiS ->
+        oidx <> sidx ->
+        getDir oidx (removeSharer sidx dir) = getDir oidx dir.
+    Proof.
+      dir_crush.
+      - exfalso; apply removeOnce_In_2 in i; auto.
+      - exfalso; elim n.
+        apply removeOnce_In_1; assumption.
+    Qed.
+
+    Lemma getDir_LastSharer_eq:
+      forall sidx dir,
+        dir_st dir = msiS ->
+        LastSharer dir sidx ->
+        getDir sidx dir = msiS.
+    Proof.
+      unfold LastSharer; dir_crush.
+      rewrite H0 in *; firstorder idtac.
+    Qed.
+
+    Lemma getDir_LastSharer_neq:
+      forall oidx sidx dir,
+        getDir sidx dir = msiS ->
+        LastSharer dir sidx -> oidx <> sidx ->
+        getDir oidx dir = msiI.
+    Proof.
+      unfold LastSharer; dir_crush.
+      rewrite H0 in *; dest_in; exfalso; auto.
+    Qed.
+
+    Lemma getDir_S_sharer:
+      forall dir,
+        dir.(dir_st) = msiS ->
+        forall oidx,
+          In oidx dir.(dir_sharers) ->
+          getDir oidx dir = msiS.
+    Proof. dir_crush. Qed.
+
+    Lemma getDir_S_non_sharer:
+      forall dir,
+        dir.(dir_st) = msiS ->
+        forall oidx,
+          ~ In oidx dir.(dir_sharers) ->
+          getDir oidx dir = msiI.
+    Proof. dir_crush. Qed.
+
+    Lemma getDir_st_I:
+      forall dir,
+        dir.(dir_st) = msiI ->
+        forall oidx, getDir oidx dir = msiI.
+    Proof. dir_crush. Qed.
+
+    Lemma getDir_st_sound:
+      forall dir oidx,
+        msiS <= getDir oidx dir ->
+        getDir oidx dir <= dir.(dir_st).
+    Proof. dir_crush. Qed.
+
+    Lemma getDir_setDirI:
+      forall oidx, getDir oidx setDirI = msiI.
+    Proof. dir_crush. Qed.
+
+    Lemma getDir_setDirS_I_imp:
+      forall oidx shs, getDir oidx (setDirS shs) = msiI -> ~ In oidx shs.
+    Proof. dir_crush. Qed.
+
+    Lemma getDir_setDirS_S_imp:
+      forall oidx shs, getDir oidx (setDirS shs) = msiS -> In oidx shs.
+    Proof. dir_crush. Qed.
+
+    Lemma getDir_setDirS_sound:
+      forall oidx shs, getDir oidx (setDirS shs) <= msiS.
+    Proof. dir_crush. Qed.
+
+    Lemma getDir_setDirS_in:
+      forall oidx shs, In oidx shs -> getDir oidx (setDirS shs) = msiS.
+    Proof. dir_crush. Qed.
+
+    Lemma getDir_setDirS_not_in:
+      forall oidx shs, ~ In oidx shs -> getDir oidx (setDirS shs) = msiI.
+    Proof. dir_crush. Qed.
+
+    Lemma getDir_setDirS_eq:
+      forall oidx, getDir oidx (setDirS [oidx]) = msiS.
+    Proof. dir_crush. Qed.
+
+    Lemma getDir_setDirM_eq:
+      forall oidx, getDir oidx (setDirM oidx) = msiM.
+    Proof. dir_crush. Qed.
+
+    Lemma getDir_setDirM_neq:
+      forall oidx eidx, eidx <> oidx -> getDir oidx (setDirM eidx) = msiI.
+    Proof. dir_crush. Qed.
+
+    Lemma getDir_excl_eq:
+      forall dir eidx,
+        eidx = dir.(dir_excl) ->
+        dir.(dir_st) = msiM ->
+        getDir eidx dir = dir.(dir_st).
+    Proof. dir_crush. Qed.
+
+    Lemma getDir_excl_neq:
+      forall dir eidx,
+        eidx = dir.(dir_excl) ->
+        dir.(dir_st) = msiM ->
+        forall oidx,
+          oidx <> eidx ->
+          getDir oidx dir = msiI.
+    Proof. dir_crush. Qed.
+
+  End Facts.
+
+End Directory.
